=== PAGE 93 ===
Solving Systems of Linear Inequalities

A system of linear inequalities in two variables or simply a system of inequalities consists of two or more linear inequalities in the same variable. As:

x - y > 9   Inequality I  }
2x + y < 9  Inequality II } A

A solution of a system of linear inequalities is an ordered pair that is a solution of each inequality in the system. For example, (7, -6) is a solution of the system A.

The graph of a system of linear inequalities is the graph of all solutions of the system.

Example: Graph the system of inequalities:
  x + y > -2
  3x - y >= -6

Solution:

Step I: Graph both inequalities in the same coordinate plane.

Step II: Find the solution of each inequality. Preferably taking (0, 0) as test point to decide the solution region.

Step III: The graph of the system in the intersection of the two half planes. Which is shaded red.

Check: Choose a point in the region such as (0, 1). To check this solution, substitute 0 for x and 1 for y into each inequality.

  Inequality I:                Inequality II:
  x + y > -2                  3x - y >= -6
  0 + 1 > -2                  3(0) - 1 >= -6
  1 > -2  True                -1 >= -6  True

This dark shaded region is a solution of these inequalities.

Key Fact:
- Graph each inequality in the cartesian plane.
- Find the intersection of the half planes.
- The graph of system is the intersection.

Unit 04: Linear and Quadratic Inequalities          93          National Book Foundation
---
DIAGRAM: The page contains a coordinate plane graph showing the system of two linear inequalities. Two lines are drawn: the line for x + y = -2 (drawn as a dashed line since the inequality is strict >) and the line for 3x - y = -6 (drawn as a solid line since the inequality is >=). The coordinate plane has x-axis and y-axis with grid lines visible. The region above the line x + y = -2 and the region below (or on) the line 3x - y = -6 are shaded. The intersection of these two shaded regions -- the area where both inequalities are satisfied simultaneously -- is shaded darker (described as "shaded red" in the text). This darker overlapping region represents the solution set of the system. The graph shows the feasible region as a wedge-shaped area. An annotation with an arrow points to the dark shaded region with the label "This dark shaded region is a solution of these inequalities."

=== PAGE 97 ===
05

Algebraic Fractions

After studying this unit students will be able to:
- Describe rational expression.
- Factorize and simplify rational expression.
- Demonstrate manipulation of algebraic fractions.
- Performs operations on rational expressions.
- Solve rational equations.
- Apply the concept of rational equations to real world problems.

Use of letters to represent an unknown quantity was introduced by "Rene Descartes", a French Mathematician, in 1637. Today 'x' is used by most nations as the standard letter for a single unknown. In fact x-rays were so named because the scientists who discovered them did not know what they were and thus labeled them the 'unknown rays' or x-rays. Algebra is basically an extension of Arithmetic.

X-ray

A factory worker wants to work overtime to fulfill his basic necessities of life. The factory owner has decided to give him Rs. 60 per hour for working extra. But sometimes he does not have enough time to work overtime daily. So he cannot find his accurate monthly income for working extra. If we represent overtime of the worker in hours for a month by an unknown quantity say 't', then we can say that his salary for working overtime will be '60t'.
---
DIAGRAM: The page contains two photographs. The first photograph (upper right area, labeled "X-ray") shows an X-ray image of a human hand, displaying the bones of the fingers, palm, and wrist in the characteristic white-on-dark style of medical X-ray imaging. The second photograph (lower right area) shows a factory worker operating machinery in a dimly lit industrial setting, illustrating the real-world context of the word problem about overtime work.

=== PAGE 103 ===
(iv) 3x - y + 1/z  if x = -1/2, y = 3, z = -1/3

(v) 0.1d^2 + 0.01d + 1  if d = -0.2   (vi) (4/7)b^3 - 3(1/2)b^2 + b - 3  if b = 1/2

3.  If nth triangular number is represented by T(n) = n(n+1)/2, then find 100th triangular number.

4.  If P(x) = x^2 + 2x - 15, D(x) = x - 3 and Q(x) = x + 5, show that P(2)/Q(2) = D(2).

5.  If g(x) = 1/(2x^2) + x/2 + 2, find g(-1/3).

6.  The volume of a basketball (sphere) is approximately 38808 cm^3. The radius 'r' of the ball is given by

    r = cube_root(3v / 4pi), where v is its volume.

    Determine the radius of that ball. (take pi = 22/7)

Basic Operations on Algebraic Fractions

Operations with rational numbers and rational algebraic expressions are very similar. A rational number can be expressed as the quotient of two integers. A rational algebraic expression can be expressed as the quotient of two polynomials. In either case, the denominator can never be 0.

Rational Numbers: 3/11, 27/100, -7/25, 61/-89

Rational Algebraic Expressions: 5/x, y/10, 2x/(x-5), (y^2 - 36)/(y+6), (x^2 - 6x + 5)/(5x/(x+1))

If P and Q are any two algebraic expressions then P/Q is called an algebraic fraction,

where Q != 0  e.g., (a - b)/(a^2 + 2ab + b^2)

To write a fraction in simplest form, we divide both the numerator and denominator by their greatest common factor (GCD).

Unit 05: Algebraic Fractions          103          National Book Foundation
---
DIAGRAM: The page contains an illustration of a basketball (sphere) positioned to the right of problem 6. The basketball is drawn with characteristic curved seam lines on its surface, showing the typical pattern of a basketball. It appears as a shaded spherical object with visible panel lines, used to illustrate the context of the volume/radius problem.

=== PAGE 105 ===
Multiplication of Algebraic Expressions

Multiplication of algebraic expression can be explained with the help of following examples.

Example: Find the product of (x^2 - 9)/(x^2 + 2x) and x/(x + 3).

Solution:
  (x^2 - 9)/(x^2 + 2x) * x/(x + 3)
  = (x + 3)(x - 3)/(x(x + 2)) * x/(x + 3)
  = (x - 3)/(x + 2)

Example: Multiply x^2 - x - 20 by 3/(x^2 + 4x).

Solution: (x^2 - x - 20) * 3/(x^2 + 4x)

= (x^2 - 5x + 4x - 20) * 3/(x^2(x + 4))

= (x - 5)(x + 4) * 3/(x^2(x + 4))  =  (3x - 15)/x^2

Key Fact:
For all rational expressions
a/b and c/d, b != 0, d != 0:

a/b * c/d = ac/bd,  a/b / c/d = a/b * d/c = ad/bc

Division of Algebraic Expressions

The process of dividing any two algebraic expressions is explained with the help of following examples.

Example: Divide (2x^2 - 11x - 21)/(x^2 - 49) by (2x + 3)/(x + 7).

Solution:
  (2x^2 - 11x - 21)/(x^2 - 49) / (2x + 3)/(x + 7)
  = (2x^2 - 14x - 3x - 21)/((x)^2 - (7)^2) * (x + 7)/(2x + 3)
  = (2x(x - 7) + 3(x - 7))/((x + 7)(x - 7)) * (x + 7)/(2x + 3)
  = (x - 7)(2x + 3)/((x + 7)(x - 7)) * (x + 7)/(2x + 3)
  = 1

Complex Algebraic Expressions

For simplifying the complex algebraic expression involving addition, subtraction, multiplication and division, we apply the BODMAS rule similar to arithmetic expression.

Unit 05: Algebraic Fractions          105          National Book Foundation
---
DIAGRAM: No diagram on this page.

=== PAGE 107 ===
  = [ a(a - b)/(a^2 - ab + b^2) ] * [ (a + b)^2 - 3ab ] / [ (a + b)^2 - 4ab ]

  = [ a(a - b)/(a^2 - ab + b^2) ] * [ a^2 + 2ab + b^2 - 3ab ] / [ a^2 + 2ab + b^2 - 4ab ]

  = [ a(a - b)/(a^2 - ab + b^2) ] * [ (a^2 + b^2 - ab) / (a^2 + b^2 - 2ab) ]

  = [ a(a - b) ] / [ a^2 - 2ab + b^2 ]

  = [ a(a - b) ] / [ (a - b)^2 ]

  = a / (a - b)

Another method for simplifying a complex rational expression involves first adding or subtracting, as necessary, to get one rational expression in the numerator and one rational expression in the denominator. The problem is thereby simplified to one involving the division of two expressions.

Example: Simplify.  (3/x - 2/x^2) / (1/(x - 2) + 1/x^2)

Solution:
  (3/x - 2/x^2) / (1/(x - 2) + 1/x^2)

  = (3x - 2)/(x^2) / (x^2(x - 2)),  taking LCM

  = (3x - 2)/x^2 * x^2(x - 2)/(3x^2 + x - 2),  to divide, multiply by the reciprocal of the divisor.

  = (3x - 2)/x^2 * x^2(x - 2)/(3x^2 + 3x - 2x - 2)

  = (3x - 2)/x^2 * x^2(x - 2)/((3x - 2)(x + 1)),  factoring

  = (x - 2)/(x + 1),  removing a common factor from numerator and denominator.

Unit 05: Algebraic Fractions          107          National Book Foundation
---
DIAGRAM: No diagram on this page.
